% Author: JÃ¸rn Olav Jensen

\newpage
\section{Suggested solutions: Sinusoidal Signals}
\begin{enumerate}
  % Exercise 1
  \item If $x_{\text{noise}}(t)=\cos(\omega t+\phi)$ and $x_{\text{cancel}}(t)=\cos(\omega t+\phi_{c})$ and:
        \[ x_{\text{noise}}(t)+x_{\text{cancel}}(t)=0, \]
        then we must have:
        \[ \cos(\omega t+\phi)+\cos(\omega t+\phi_{c})=0, \]
        for all $t$. The phase doesn't depend on $t$, so it is the same for every $t\in\mathbb{R}$, in particular for $t=0$ so:
        \begin{align*}
          \cos(\phi)  & =-\cos(\phi_{c}),     \\
          \cos(\phi)  & =\cos(\pi -\phi_{c}), \\
          \phi+2\pi k & =\pi-\phi_{c}+2\pi l,
        \end{align*}
        for $k,l\in\mathbb{Z}$, which gives $\phi_{c}=\pi-\phi+2\pi(l-k)=\pi-\phi+2\pi m$,
        where $m\in\mathbb{Z}$. Take $m=0$ to obtain a simple solution, which gives $\phi_{c}=\pi -\phi$.
        Hence, the canceling signal must be of the form:
        \[ x_{\text{cancel}}(t)=\cos(\omega t+(\pi-\phi)). \]
        A simple test program to verify this is shown in Listing \ref{cancel}
        with an arbitrary choice of $\omega$, $\phi$ and $m$.
        If the code is run, two signals of opposite amplitude are shown,
        which cancel out when added, as hoped.
        \lstinputlisting[language=Python, caption={Noise canceling signal}, label=cancel, linerange={0-25}]{ch06/code/ex6.1.py}

  % Exercise 2
  \item Have that:
        \[ a\cos(\omega t)+b\sin(\omega t)=\frac{a}{2}(e^{i\omega t}+e^{-i\omega t})+\frac{b}{2i}(e^{i\omega t}-e^{-i\omega t}), \]
        or written out:
        \[ a\cos(\omega t)+b\sin(\omega t)=\frac{a}{2}e^{i\omega t}+\frac{a}{2}e^{-i\omega t}+\frac{b}{2i}e^{i\omega t}-\frac{b}{2i}e^{-i\omega t}. \]
        Using the phasor summation property we have:
        \[ X = \sum_{n}X_{n} = \frac{a}{2}+\frac{b}{2i}=\frac{1}{2}(a-bi), \]
        and
        \[ Y = \sum_{m}Y_{m} = \frac{a}{2}-\frac{b}{2i}=\frac{1}{2}(a+bi). \]
        Then we have that:
        \begin{align*}
          |X| & =\sqrt{\frac{1}{4}(a^{2}+b^{2})}=\frac{1}{2}\sqrt{a^{2}+b^{2}}, \\
          |Y| & =\sqrt{\frac{1}{4}(a^{2}+b^{2})}=\frac{1}{2}\sqrt{a^{2}+b^{2}},
        \end{align*}
        and
        \begin{align*}
          \angle X & =\arctan\left(\frac{-b}{a}\right)=\phi, \\
          \angle Y & =\arctan\left(\frac{b}{a}\right).
        \end{align*}
        Then the whole expression can be rewritten as:
        \begin{align*}
          a\cos(\omega t)+b\sin(\omega t) & =\frac{1}{2}\sqrt{a^{2}+b^{2}}e^{i\phi}e^{i\omega t}+\frac{1}{2}\sqrt{a^{2}+b^{2}}e^{-i\phi}e^{-i\omega t}, \\
                                          & =\frac{1}{2}\sqrt{a^{2}+b^{2}}e^{i(\omega t+\phi)}+\frac{1}{2}\sqrt{a^{2}+b^{2}}e^{-i(\omega t+\phi)},      \\
                                          & =\sqrt{a^{2}+b^{2}}\left[\frac{1}{2}\left(e^{i(\omega t+\phi)}+e^{-i(\omega t+\phi)}\right)\right],         \\
                                          & =\sqrt{a^{2}+b^{2}}\cos(\omega t+\phi),                                                                     \\
                                          & =A\cos(\omega t+\phi).
        \end{align*}
        Here $A=\sqrt{a^{2}+b^{2}}$ and $\phi=-\arctan(b/a)$, where $\arctan(b/a)$
        should give the angle corresponding to which quadrant the point $(a,b)$ lies in the $xy$-plane.

  % Exercise 3
  \item Consider the signal:
        \[ x(t) = \cos(\omega_{1}t)\sin(\omega_{2}t), \]
        which we can write as:
        \[ x(t) = \frac{1}{2}(e^{i\omega_{1}t}+e^{-i\omega_{1} t})\frac{1}{2i}(e^{i\omega_{2}t}-e^{-i\omega_{2}t})=\frac{1}{4i}[e^{i(\omega_{1}+\omega_{2})t}-e^{i(\omega_{1}-\omega_{2})t}+e^{i(-\omega_{1}+\omega_{2})t}-e^{i(-\omega_{1}-\omega_{2})t}]. \]
        Collecting terms we get:
        \begin{align*}
          x(t) & =\frac{1}{4i}[e^{i(\omega_{1}+\omega_{2})t}-e^{-i(\omega_{1}+\omega_{2})t}]+\frac{1}{4i}[e^{i(-\omega_{1}+\omega_{2})t}-e^{-i(-\omega_{1}+\omega_{2})t}], \\
               & =\frac{1}{2}\sin((\omega_{1}+\omega_{2})t)+\frac{1}{2}\sin((\omega_{2}-\omega_{1})t).
        \end{align*}
        This yields the values $a=1/2$ and $b=1/2$, while $\omega_{3}=\omega_{1}+\omega_{2}$ and $\omega_{4}=\omega_{2}-\omega_{1}$.

  % Exercise 4
  \item The plane wave:
        \[ E(x,t) = E_{0}e^{i(kx+\omega t)}\partial_{y} \]
        is a solution to the wave equation. Consider the real part $\Re\{E(x,t)\}$:
        \[ \Re\{E(x,t)\} = \frac{1}{2}[E(x,t)+E^{*}(x,t)]=\frac{1}{2}E_{0}(e^{i(kx+\omega t)}+e^{-i(kx+\omega t)})\partial_{y}=E_{0}\cos(kx+\omega t)\partial_{y}. \]
        Recall that the wave equation is:
        \[ \partial_{t}^{2}E-\frac{1}{\mu_{0}\epsilon_{0}}\nabla^{2}E=0, \]
        which gives:
        \[ -\omega^{2}E_{0}\cos(kx+\omega t)\partial_{y}+\frac{1}{\mu_{0}\epsilon_{0}}k^{2}E_{0}\cos(kx+\omega t)\partial_{y}=E_{0}\left(\frac{1}{\mu_{0}\epsilon_{0}}k^{2}-\omega^{2}\right)\cos(kx+\omega t)\partial_{y}=0, \]
        since $k^{2}c^{2}-\omega^{2}=0$, as $c=\sqrt{1/\mu_0\epsilon_0}$. In conclusion, the signal:
        \[ \Re\{E(x,t)\} = E_{0}\cos(kx+\omega t)\partial_{y}, \]
        is a solution to the wave equation.

  % Exercise 5
  \item If we have an arbitrary number of solutions to the wave equation, each with different
        phasors $E_{n}$ and different angular frequencies $\omega_{n}$. Then a superposition:
        \[ E(x,t) = \sum_{n}E_{n}e^{i(\omega_{n}/c)x}e^{i\omega_{n}t}\partial_{y}, \]
        is also a solution. This follows by the linearity of the wave equation.

  % Exercise 6
  \item The code from the notes has been modified such that the output signal has a frequency of approximately 42.0 Hz.
        \lstinputlisting[language=Python, caption={Adding frequencies}, label=sig42, linerange={0-33}]{ch06/code/ex6.6.py}
        Running the code in Listing \ref{sig42} yields the following output:
        \begin{figure}[h!]
          \centering
          \includegraphics[scale=1.0]{ch06/figures/ex6a.png}
          \caption{Signal with 42 Hz frequency}
        \end{figure}

  % Exercise 7
  \item The following code is a modification that multiplies the signal with a periodic 5.0 Hz signal:
        \begin{itemize}
          % Exercise 7a)
          \item[a)] Listing \ref{sig42_mod} provides a suggested solution.
                \lstinputlisting[language=Python, caption={Modifying signals}, label=sig42_mod, linerange={0-23}]{ch06/code/ex6.7a.py}
                Running Listing \ref{sig42_mod} produces Figure \ref{fig:ex6b}.
                \begin{figure}[h!]
                  \centering
                  \includegraphics[width=12.5cm, height=9.5cm]{ch06/figures/ex6b.png}
                  \caption{Original and modified guitar signal}
                  \label{fig:ex6b}
                \end{figure}

          % Exercise 7b)
          \item[b)]
                Adding the following code to Listing \ref{sig42_mod} will save the result as an audio file.
\begin{lstlisting}[language=Python, caption=Saving an audiofile, label=save_audio]
out = 0.9*out/np.max(np.abs(out)) 
    
# Multiply the signals.
out2 = x*n.cos(2.0*n.pi*time_vec*2.5)
    
# Write compressed output to wav file.
sio.write("guitar_leslie.wav", sample_rate, np.array(out, dtype=np.float32))
\end{lstlisting}
                Listening to the audio file, we hear that the guitar sound has a wavy oscillating effect.

          % Exercise 7c)
          \item[c)]
                Based on the previous task, the result of multiplying with a 2.5 Hz signal will result in 
                the same effect, but the oscillation will be slower. After testing this 
                by running Listing \ref{save_audio} this is exactly what happens.
        \end{itemize}

\end{enumerate}
