\newpage
\section{Exercises: Fourier Transform}
\begin{enumerate}
\item A rectangular signal is defined as:
\begin{equation}
    x(t) = u\left(t+1\right)-u\left(t-1\right)
\end{equation}
\begin{enumerate}[a)]
\item Sketch a plot of $x(t)$. How long is the rectangular pulse $x(t)$?
\item This signal is scaled in time as follows $y(t) = x(2t)$. Sketch a plot of the signal $y(t)$. How long is the rectangular pulse $y(t)$?
\item Evaluate the Fourier transforms of these functions: $\hat{x}(\omega)=\mathcal{F}\{x(t)\}$ and $\hat{y}(\omega)=\mathcal{F}\{y(t)\}$ using the definition of the Fourier transform.
\item How wide are the sinc functions $\hat{x}(\omega)$ and $\hat{y}(\omega)$? You can use, e.g., the spacing between the first zero crossings of the sinc function as a measure of width. Does this agree with Equation \ref{eq:timescale_ft_pair}?
\end{enumerate}

\item Find the Fourier transforms of these signals:
\begin{enumerate}[a)]
\item $x(t)=\delta(t+2)+\delta(t)+\delta(t-2)$ \\Hint: linearity and time shift properties.
\item $x(t)=\frac{\sin(100\pi [t-2])}{\pi (t-2)}$ \\Hint: time shift property.
\item $x(t)=e^{-t}u(t) - e^{-t} u(t-4)$ \\Hint: look at the derivation of the Fourier transform of $e^{-\beta t} u(t)$.
\end{enumerate}
Note that there are more than one way to solve the Fourier transforms!

\item Find the inverse Fourier transform for the following:
\begin{enumerate}[a)]
\item $\hat{x}(\omega)= 2 + \cos(\omega)$
\item $\hat{x}(\omega) = \frac{1}{1+i\omega} - \frac{1}{2+i\omega}$
\item $\hat{x}(\omega) = i \delta(\omega - 100\pi) - i\delta(\omega + 100\pi)$.
\end{enumerate}

\item Use known Fourier transform pairs together with the properties of the Fourier transform to complete the following Fourier transform pairs:
  \begin{enumerate}[a)]
  \item $x(t) = u(t+3)u(3-t) \xleftrightarrow{\mathcal{F}} \hat{x} = ?$
  \item $x(t) = \sin(4\pi t) \sin(50 \pi t)  \xleftrightarrow{\mathcal{F}} \hat{x} = ?$
  \item $x(t) = \frac{\sin(4\pi t)}{\pi t} \sin(50 \pi t)  \xleftrightarrow{\mathcal{F}} \hat{x} = ?$
  \item $x(t) = ?  \xleftrightarrow{\mathcal{F}} \hat{x} = \cos^2(\omega)$    
  \end{enumerate}


\item Let $\hat{x}(\omega)$ be the Fourier transform of $x(t)$. Prove that if $y(t)=x(t-\tau)$, then $\hat{y}(\omega)=e^{-i\tau}\hat{x}(\omega)$. 
  
  
  
  
\end{enumerate}
